theories/Pre_orders/Must/Must.v
@@ -401,24 +401,24 @@ Notation "p ≼₁ q" := (bhv_pre_cond1 p q) (at level 70).
   Each state can only reduce for finitely many preactions *)
 Class PreExtAction `{H : ExtAction A} {P : Type} `{Countable PreAct} {𝝳 : A → PreAct} (LtsP : @gLts P A H):=
   MkPreExtAction {
-      preactions_of : P -> gset PreAct; (* finite subset_of A *) 
+      pre_co_actions_of : P -> gset PreAct; (* finite subset_of A *) 
 
-      preactions_of_spec (μ : A) (p : P) : μ ∈ lts_acc_set_of p <-> (𝝳 μ) ∈ (preactions_of p) ;
+      preactions_of_spec (μ : A) (p : P) : μ ∈ co_actions_of p <-> (𝝳 μ) ∈ (pre_co_actions_of p) ;
   }.
 
-Definition bhv_pre_cond2 `{PreA_countable : Countable PreA} `{
-  LtsP : @gLts P A H, PreAP : @PreExtAction A H P PreA _ _ 𝝳P LtsP,
-  LtsQ : @gLts Q A H, PreAQ : @PreExtAction A H Q PreA _ _ 𝝳Q LtsQ}
+Definition bhv_pre_cond2 `{
+  LtsP : @gLts P A H, PreAP : @PreExtAction A H P PreA PreA_eq PreA_countable 𝝳 LtsP,
+  LtsQ : @gLts Q A H, PreAQ : @PreExtAction A H Q PreA PreA_eq PreA_countable 𝝳 LtsQ}
   (p : P) (q : Q) :=
   forall s q',
     p ⇓ s -> q ⟹[s] q' -> q' ↛ ->
-    ∃ p', p ⟹[s] p' /\ p' ↛ /\ (preactions_of p' ⊆ preactions_of q').
+    ∃ p', p ⟹[s] p' /\ p' ↛ /\ (pre_co_actions_of p' ⊆ pre_co_actions_of q').
 
 Notation "p ≼₂ q" := (bhv_pre_cond2 p q) (at level 70).
 
 Definition bhv_pre `{PreA_countable : Countable PreA} `{
-  LtsP : @gLts P A H, PreAP : @PreExtAction A _ P PreA _ _ 𝝳P LtsP,
-  LtsQ : @gLts Q A H, PreAQ : @PreExtAction A _ Q PreA _ _ 𝝳Q LtsQ}
+  LtsP : @gLts P A H, PreAP : @PreExtAction A _ P PreA _ _ 𝝳 LtsP,
+  LtsQ : @gLts Q A H, PreAQ : @PreExtAction A _ Q PreA _ _ 𝝳 LtsQ}
     (p : P) (q : Q) := 
       p ≼₁ q /\ p ≼₂ q.
 
